Frontiers - implementation with linked list

Frontier.dfy
@@ -67,94 +67,95 @@ method FrontierIter<T>(tree: BT<T>, io: IO<T>)
 	modifies io
 	ensures io.omega == old(io.omega) + Frontier(tree)
 {
-	// We chose to use a sequence because of the following (in no particular order):
-	// 1. Trying to use an array which grows dynamically was giving us trouble.
-	//    We didn't learn how to use an array as local variable.
-	//    We lack `reads` and `modifies` permissions on the array to actually
-	//    make use of it and we only saw how to do that when the array is passed
-	//    as an argument to a method.
-	//    And we can't do that because the pointer also has to change dynamically
-	//    in order to grow dynamically which then implies it has to be a local variable.
-	// 2. Problems with writing a function to calculate the maximum size
-	//    will be used by the stack:
-	//    1. It will be complex to prove to Dafny that the algorthim never exceeds the
-	//       the array size.
-	//    2. But not only that, an even bigger issue is that doing so will never
-	//       acutally be done in practice because why do so when using an array which
-	//       grows dynamically is efficient and is simpler.
-	//       So doing so is just for the sake of doing so.
+	// The implementation is efficient because each operation of the stack manipulation is O(1).
 
-	// Why the stack grows towards the beginning rather than the end:
-	// 1. We're using a sequence anyway so this doesn't matter.
-	// 2. It makes an algorithm which is easier to prove it's correctness.
-	// 3. It seems that you had that solution in mind when making this excerise,
-	//    indicated by both the lecture and the `Frontiers` function which
-	//    takes the first item of the sequence.
-
-	var stack := [tree]; // grows towards the beginning of the sequence
-	while stack != []
+	var stack : List<BT<T>> := Cons(tree, Empty); // grows towards the beginning
+	while stack != Empty
 		invariant LoopInv(tree, stack, io.omega, old(io.omega))
 		decreases ForestSize(stack)
 	{
-		ghost var s := stack;
 		ghost var V0 := ForestSize(stack);
 
-		assert s != [];
-		assert LoopInv(tree, s, io.omega, old(io.omega));
+		assert stack != Empty;
+		assert LoopInv(tree, stack, io.omega, old(io.omega));
 
-		// This generates a compile error for some reason
-		// var t;
-		// t, stack := stack[0], stack[1..];
-		var t := stack[0];
-		stack := stack[1..];
-
-		assert s == [t] + stack;
-		assert LoopInv(tree, s, io.omega, old(io.omega));
-
-		match t
+		match stack
 		{
-			case Tip(x) =>
+			case Cons(t, s) =>
 			{
-				assert s == [t] + stack;
-				assert LoopInv(tree, s, io.omega, old(io.omega));
-				assert t == Tip(x);
-				// ==>?
-				EnsureInvTip(tree, stack, s, t, x, io.omega, old(io.omega));
-				assert LoopInv(tree, stack, io.omega + [x], old(io.omega)); // maintaining the loop invariant
+				assert stack == Cons(t, s) != Empty;
+				assert LoopInv(tree, stack, io.omega, old(io.omega));
 
-				io.Output(x);
-				assert LoopInv(tree, stack, io.omega, old(io.omega)); // maintaining the loop invariant
-				assert 0 <= ForestSize(stack) < V0; // the loop termination
-			}
-			case Node(t1, t2) =>
-			{
-				assert s == [t] + stack;
-				assert LoopInv(tree, s, io.omega, old(io.omega));
-				assert t == Node(t1, t2);
-				// ==>?
-				EnsureInvNode(tree, stack, s, t, t1, t2, io.omega, old(io.omega));
-				assert LoopInv(tree, [t1, t2] + stack, io.omega, old(io.omega));
+				match t
+				{
+					case Tip(x) =>
+					{
+						assert stack == Cons(t, s) != Empty;
+						assert LoopInv(tree, stack, io.omega, old(io.omega));
+						assert t == Tip(x);
+						// ==>?
+						EnsureInvTip(tree, stack, s, t, x, io.omega, old(io.omega));
+						EnsureDecreaseTip(stack, s, t, x);
+						assert LoopInv(tree, s, io.omega + [x], old(io.omega));
+						assert 0 <= ForestSize(s) < V0;
 
-				stack := [t1, t2] + stack;
-				assert LoopInv(tree, stack, io.omega, old(io.omega)); // maintaining the loop invariant
-				assert 0 <= ForestSize(stack) < V0; // the loop termination
-			}
-		}
+						io.Output(x);
+
+						assert LoopInv(tree, s, io.omega, old(io.omega));
+						assert 0 <= ForestSize(s) < V0;
+					}
+					case Node(t1, t2) =>
+					{
+						assert stack == Cons(t, s) != Empty;
+						assert LoopInv(tree, stack, io.omega, old(io.omega));
+						assert t == Node(t1, t2);
+						// ==>?
+						EnsureInvNode(tree, stack, s, t, t1, t2, io.omega, old(io.omega));
+						EnsureDecreaseNode(stack, s, t, t1, t2);
+						assert LoopInv(tree, Cons(t1, Cons(t2, s)), io.omega, old(io.omega));
+						assert 0 <= ForestSize(Cons(t1, Cons(t2, s))) < V0;
+
+						s := Cons(t1, Cons(t2, s));
+
+						assert LoopInv(tree, s, io.omega, old(io.omega));
+						assert 0 <= ForestSize(s) < V0;
+					}
+				}
+
+				assert LoopInv(tree, s, io.omega, old(io.omega));
+				assert 0 <= ForestSize(s) < V0;
+				stack := s;
+				assert LoopInv(tree, stack, io.omega, old(io.omega));
+				assert 0 <= ForestSize(stack) < V0;
+			} // end case Cons()
+		} // end match
 
 		assert LoopInv(tree, stack, io.omega, old(io.omega)); // maintaining the loop invariant
 		assert 0 <= ForestSize(stack) < V0; // the loop termination
 	}
 
 	assert LoopInv(tree, stack, io.omega, old(io.omega)); // from the loop invariant
-	assert stack == []; // from the negation of the loop guard
+	assert stack == Empty; // from the negation of the loop guard
 	// ==>
 	EnsurePostCondition(tree, stack, io.omega, old(io.omega));
 	assert io.omega == old(io.omega) + Frontier(tree);
 }
 
-predicate LoopInv<T>(tree: BT<T>, forest: seq<BT<T>>, omega: seq<T>, old_omega: seq<T>)
+datatype List<T> = Empty | Cons(T, List<T>)
+
+function FrontiersList<T>(forest: List<BT<T>>): seq<T>
+	decreases forest
 {
-	omega + Frontiers(forest) == old_omega + Frontier(tree)
+	match forest
+	{
+		case Empty => []
+		case Cons(tree, forest') => Frontier(tree) + FrontiersList(forest')
+	}
+}
+
+predicate LoopInv<T>(tree: BT<T>, forest: List<BT<T>>, omega: seq<T>, old_omega: seq<T>)
+{
+	omega + FrontiersList(forest) == old_omega + Frontier(tree)
 }
 
 function TreeSize<T>(tree: BT<T>): nat
@@ -168,35 +169,54 @@ function TreeSize<T>(tree: BT<T>): nat
 	}
 }
 
-function ForestSize<T>(forest: seq<BT<T>>): nat
+function ForestSize<T>(forest: List<BT<T>>): nat
 	decreases forest
 	ensures ForestSize(forest) >= 0
 {
-	if forest == [] then 0
-	else TreeSize(forest[0]) + ForestSize(forest[1..])
+	match forest
+	{
+		case Empty => 0
+		case Cons(tree, forest') => TreeSize(tree) + ForestSize(forest')
+	}
 }
 
-lemma EnsureInvTip<T>(tree: BT<T>, stack: seq<BT<T>>, s: seq<BT<T>>, t: BT<T>, x: T, omega: seq<T>, old_omega: seq<T>)
-	requires s == [t] + stack
-	requires LoopInv(tree, s, omega, old_omega)
+lemma EnsureInvTip<T>(tree: BT<T>, stack: List<BT<T>>, s: List<BT<T>>, t: BT<T>, x: T, omega: seq<T>, old_omega: seq<T>)
+	requires stack == Cons(t, s)
+	requires LoopInv(tree, stack, omega, old_omega)
 	requires t == Tip(x)
 	
-	ensures LoopInv(tree, stack, omega + [x], old_omega)
+	ensures LoopInv(tree, s, omega + [x], old_omega)
 {
 }
 
-lemma EnsureInvNode<T>(tree: BT<T>, stack: seq<BT<T>>, s: seq<BT<T>>, t: BT<T>, t1: BT<T>, t2: BT<T>, omega: seq<T>, old_omega: seq<T>)
-	requires s == [t] + stack
-	requires LoopInv(tree, s, omega, old_omega)
+lemma EnsureDecreaseTip<T>(stack: List<BT<T>>, s: List<BT<T>>, t: BT<T>, x: T)
+	requires stack == Cons(t, s)
+	requires t == Tip(x)
+	
+	ensures 0 <= ForestSize(s) < ForestSize(stack)
+{
+}
+
+lemma EnsureInvNode<T>(tree: BT<T>, stack: List<BT<T>>, s: List<BT<T>>, t: BT<T>, t1: BT<T>, t2: BT<T>, omega: seq<T>, old_omega: seq<T>)
+	requires stack == Cons(t, s)
+	requires LoopInv(tree, stack, omega, old_omega)
 	requires t == Node(t1, t2)
 	
-	ensures LoopInv(tree, [t1, t2] + stack, omega, old_omega)
+	ensures LoopInv(tree, Cons(t1, Cons(t2, s)), omega, old_omega)
 {
 }
 
-lemma {:induction false} EnsurePostCondition<T>(tree: BT<T>, stack: seq<BT<T>>, omega: seq<T>, old_omega: seq<T>)
+lemma EnsureDecreaseNode<T>(stack: List<BT<T>>, s: List<BT<T>>, t: BT<T>, t1: BT<T>, t2: BT<T>)
+	requires stack == Cons(t, s)
+	requires t == Node(t1, t2)
+	
+	ensures 0 <= ForestSize(Cons(t1, Cons(t2, s))) < ForestSize(stack)
+{
+}
+
+lemma {:induction false} EnsurePostCondition<T>(tree: BT<T>, stack: List<BT<T>>, omega: seq<T>, old_omega: seq<T>)
 	requires LoopInv(tree, stack, omega, old_omega)
-	requires stack == []
+	requires stack == Empty
 
 	ensures omega == old_omega + Frontier(tree)
 {
@@ -207,20 +227,33 @@ method FrontierIter'<T>(tree: BT<T>, io: IO<T>)
 	modifies io
 	ensures io.omega == old(io.omega) + Frontier(tree)
 {
-	var stack := [tree]; // grows towards the beginning of the sequence
-	while stack != []
+	var stack : List<BT<T>> := Cons(tree, Empty); // grows towards the beginning
+	while stack != Empty
 		invariant LoopInv(tree, stack, io.omega, old(io.omega))
 		decreases ForestSize(stack)
 	{
 		ghost var V0 := ForestSize(stack);
-		var t := stack[0];
-		stack := stack[1..];
-		match t
+
+		match stack
 		{
-			case Tip(x) => io.Output(x);
-			case Node(t1, t2) => stack := [t1, t2] + stack;
+			case Cons(t, s) =>
+			{
+				match t
+				{
+					case Tip(x) =>
+					{
+						io.Output(x);
+					}
+					case Node(t1, t2) =>
+					{
+						s := Cons(t1, Cons(t2, s));
+					}
+				}
+
+				stack := s;
+			}
 		}
 
-		assert 0 <= ForestSize(stack) < V0; // the loop terminates
+		assert 0 <= ForestSize(stack) < V0; // the loop termination
 	}
 }
